HoareLogic: yet another way to prove an invariant of a transition system

HoareLogic.v
@@ -119,6 +119,9 @@ Inductive hoare_triple : assertion -> cmd -> assertion -> Prop :=
   (forall h v, P h v -> I h v)
   -> hoare_triple (fun h v => I h v /\ beval b h v = true) c I
   -> hoare_triple P (While_ I b c) (fun h v => I h v /\ beval b h v = false)
+| HtAssert : forall P I : assertion,
+  (forall h v, P h v -> I h v)
+  -> hoare_triple P (Assert I) P
 | HtConsequence : forall (P Q P' Q' : assertion) c,
   hoare_triple P c Q
   -> (forall h v, P' h v -> P h v)
@@ -172,6 +175,7 @@ Infix "<-" := set (no associativity, at level 70) : cmd_scope.
 Infix ";;" := Seq (right associativity, at level 75) : cmd_scope.
 Notation "'when' b 'then' then_ 'else' else_ 'done'" := (If_ b then_ else_) (at level 75, e at level 0).
 Notation "{{ I }} 'while' b 'loop' body 'done'" := (While_ I b body) (at level 75).
+Notation "'assert' {{ I }}" := (Assert I) (at level 75).
 Delimit Scope cmd_scope with cmd.
 
 Infix "+" := plus : reset_scope.
@@ -196,7 +200,7 @@ Notation "{{ P }} c {{ Q }}" := (hoare_triple P c%cmd Q) (at level 90, c at next
 (** ** Swapping the values in two variables *)
 
 Ltac ht1 := apply HtSkip || apply HtAssign || apply HtWrite || eapply HtSeq
-            || eapply HtIf || eapply HtWhile
+            || eapply HtIf || eapply HtWhile || eapply HtAssert
             || match goal with
                | [ |- hoare_triple ?pre _ _ ] => eapply HtConsequence with (P := pre); [ | tauto | ]
                end.
@@ -209,7 +213,7 @@ Ltac ht := simplify; repeat ht1; cbv beta; propositional; subst;
            repeat match goal with
                   | [ _ : context[?a <=? ?b] |- _ ] => destruct (a <=? b); try discriminate
                   | [ H : ?E = ?E |- _ ] => clear H
-                  end; simplify; propositional; auto; try linear_arithmetic.
+                  end; simplify; propositional; auto; try equality; try linear_arithmetic.
 
 Theorem swap_ok : forall a b,
   {{_&v ~> v $! "x" = a /\ v $! "y" = b}}
@@ -338,4 +342,183 @@ Proof.
   specialize (H k); ht.
 
   cases (k ==n x $! "j"); ht.
+Qed.
+
+
+(** * An alternative correctness theorem for Hoare logic, with small-step semantics *)
+
+Inductive step : heap * valuation * cmd -> heap * valuation * cmd -> Prop :=
+| StAssign : forall h v x e,
+  step (h, v, Assign x e) (h, v $+ (x, eval e h v), Skip)
+| StWrite : forall h v e1 e2,
+  step (h, v, Write e1 e2) (h $+ (eval e1 h v, eval e2 h v), v, Skip)
+| StStepSkip : forall h v c,
+  step (h, v, Seq Skip c) (h, v, c)
+| StStepRec : forall h1 v1 c1 h2 v2 c1' c2,
+  step (h1, v1, c1) (h2, v2, c1')
+  -> step (h1, v1, Seq c1 c2) (h2, v2, Seq c1' c2)
+| StIfTrue : forall h v b c1 c2,
+  beval b h v = true
+  -> step (h, v, If_ b c1 c2) (h, v, c1)
+| StIfFalse : forall h v b c1 c2,
+  beval b h v = false
+  -> step (h, v, If_ b c1 c2) (h, v, c2)
+| StWhileFalse : forall I h v b c,
+  beval b h v = false
+  -> step (h, v, While_ I b c) (h, v, Skip)
+| StWhileTrue : forall I h v b c,
+  beval b h v = true
+  -> step (h, v, While_ I b c) (h, v, Seq c (While_ I b c))
+| StAssert : forall h v (a : assertion),
+  a h v
+  -> step (h, v, Assert a) (h, v, Skip).
+
+Hint Constructors step.
+
+Definition trsys_of (st : heap * valuation * cmd) := {|
+  Initial := {st};
+  Step := step
+|}.
+
+Definition unstuck (st : heap * valuation * cmd) :=
+  snd st = Skip
+  \/ exists st', step st st'.
+
+Lemma hoare_triple_unstuck : forall P c Q,
+  {{P}} c {{Q}}
+  -> forall h v, P h v
+                 -> unstuck (h, v, c).
+Proof.
+  induct 1; unfold unstuck; simplify; propositional; eauto.
+
+  apply IHhoare_triple1 in H1.
+  unfold unstuck in H1; simplify; first_order; subst; eauto.
+  cases x.
+  cases p.
+  eauto.
+
+  cases (beval b h v); eauto.
+
+  cases (beval b h v); eauto.
+
+  apply H0 in H2.
+  apply IHhoare_triple in H2.
+  unfold unstuck in H2; simplify; first_order.
+Qed.
+
+Lemma hoare_triple_Skip : forall P Q,
+  {{P}} Skip {{Q}}
+  -> forall h v, P h v -> Q h v.
+Proof.
+  induct 1; auto.
+Qed.
+
+Lemma hoare_triple_step : forall P c Q,
+  {{P}} c {{Q}}
+  -> forall h v h' v' c',
+      step (h, v, c) (h', v', c')
+      -> P h v
+      -> {{h''&v'' ~> h'' = h' /\ v'' = v'}} c' {{Q}}.
+Proof.
+  induct 1.
+
+  invert 1.
+
+  invert 1; ht; eauto.
+
+  invert 1; ht; eauto.
+
+  invert 1; simplify.
+
+  eapply HtConsequence; eauto.
+  propositional; subst.
+  eapply hoare_triple_Skip; eauto.
+
+  econstructor; eauto.
+
+  invert 1; simplify.
+  eapply HtConsequence; eauto; equality.
+  eapply HtConsequence; eauto; equality.
+
+  invert 1; simplify.
+  eapply HtConsequence with (P := h'' & v'' ~> h'' = h' /\ v'' = v').
+  apply HtSkip.
+  auto.
+  simplify; propositional; subst; eauto.
+
+  econstructor.
+  eapply HtConsequence; eauto.
+  simplify; propositional; subst; eauto.
+  econstructor; eauto.
+
+  invert 1; simplify.
+  eapply HtConsequence; eauto.
+  econstructor.
+  simplify; propositional; subst; eauto.
+
+  simplify.
+  eapply HtConsequence.
+  eapply IHhoare_triple; eauto.
+  simplify; propositional; subst; eauto.
+  auto.
+Qed.
+
+Theorem hoare_triple_invariant : forall P c Q h v,
+  {{P}} c {{Q}}
+  -> P h v
+  -> invariantFor (trsys_of (h, v, c)) unstuck.
+Proof.
+  simplify.
+  apply invariant_weaken with (invariant1 := fun st => {{h&v ~> h = fst (fst st)
+                                                           /\ v = snd (fst st)}}
+                                                         snd st
+                                                       {{_&_ ~> True}}).
+
+  apply invariant_induction; simplify.
+
+  propositional; subst; simplify.
+  eapply HtConsequence; eauto.
+  equality.
+
+  cases s.
+  cases s'.
+  cases p.
+  cases p0.
+  simplify.
+  eapply hoare_triple_step; eauto.
+  simplify; auto.
+
+  simplify.
+  cases s.
+  cases p.
+  simplify.
+  eapply hoare_triple_unstuck; eauto.
+  simplify; auto.
+Qed.
+
+(* A very simple example, just to show all this in action. *)
+Definition forever := (
+  "i" <- 1;;
+  "n" <- 1;;
+  {{h&v ~> v $! "i" > 0}}
+  while 0 < "i" loop
+    "i" <- "i" * 2;;
+    "n" <- "n" + "i";;
+    assert {{h&v ~> v $! "n" >= 1}}
+  done;;
+
+  assert {{_&_ ~> False}}
+  (* Note that this last assertion implies that the program never terminates! *)
+)%cmd.
+
+Theorem forever_ok : {{_&_ ~> True}} forever {{_&_ ~> False}}.
+Proof.
+  ht.
+Qed.
+
+Theorem forever_invariant : invariantFor (trsys_of ($0, $0, forever)) unstuck.
+Proof.
+  eapply hoare_triple_invariant.
+  apply forever_ok.
+  simplify; trivial.
 Qed.
